### <center>Relation Between the Displacement of the Object with its Initial and Final Velocity in UAM</center>


We already know that 
 $$S_x = v_{o_x}t  + \frac{a_xt^2}{2} \ \ \ \ \ \ \ \ \ v_{o_x}, \ a_x, \ t$$
$$S_x = \frac{v_x + v_{o_x}}{2}\cdot t \ \ \ \ \ \ \ \ \ v_{o_x}, \ v_x, \ t \ \ \ \  \ \ \ \  (2)$$

$$\begin{align}
v_x = v_{o_x} + a_xt\\
a_xt = v_x - v_{o_x}\\
\end{align}$$
$$t = \frac{ v_x - v_{o_x}}{a_x}$$
Substitute this equation into $(2)$
$$S_x = \frac{v_x + v_{o_x}}{2} \cdot \frac{ v_x - v_{o_x}}{a_x} = \frac{(v_x + v_{o_x})(v_x - v_{o_x})}{2a_x} = \frac{v_x^2 - v_{o_x}^2}{2a_x}.$$


$$\large\boxed{S_x = \frac{v_x^2 - v_{o_x}^2}{2a_x}} \ \ \ \ \ \ \ \ \ v_{o_x}, \ v_x, \ a_x$$


---

tags: #mechanics/kinematics #motion #velocity 



references: [Урок 29. Связь перемещения при РУД с начальной и конечной скоростью](https://www.youtube.com/watch?v=a-0P_qya90Y&list=PL1Us50cZo25k6lXqOyfCYiKoTvaSbYxHX&index=6)